SemVer/Lemmas.lean
@@ -1,0 +1,93 @@
+/-
+Copyright (c) 2025 Stefan Kusterer. All rights reserved.
+Released under Apache 2.0 license as described in the file LICENSE.
+-/
+
+import SemVer.Basic
+
+/-
+def a : Digits := ⟨⟨"02", rfl⟩, rfl⟩
+def b : Digits := ⟨⟨"1", rfl⟩, rfl⟩
+
+#eval a.val < b.val
+#eval b < a
+
+theorem inj_not_incr : ∃ a b : Digits, a.val < b.val ∧ b < a := by
+  let a : Digits := ⟨⟨"02", rfl⟩, rfl⟩
+  let b : Digits := ⟨⟨"1", rfl⟩, rfl⟩
+  have h1 : a.val < b.val := by simp [a,b]; decide
+  have na : 2 = a.toNat := by simp [a]; unfold toNat; simp; sorry
+  sorry
+-/
+
+/-
+TODO: Remove if not needed
+-/
+namespace Char
+
+def parseForNatBase10 : Char → ParserResult Nat
+  | '0' => .success 0
+  | '1' => .success 1
+  | '2' => .success 2
+  | '3' => .success 3
+  | '4' => .success 4
+  | '5' => .success 5
+  | '6' => .success 6
+  | '7' => .success 7
+  | '8' => .success 8
+  | '9' => .success 9
+  |  c  => .failure {message := s!"{c} is no digit", position := 0}
+
+def isDigitBase10 (chr : Char) : Bool := chr.parseForNatBase10.isSuccess
+
+def decIsDigitBase10 (chr : Char) : Decidable (chr.isDigitBase10) :=
+  if h: chr.parseForNatBase10.isSuccess then
+    isTrue (by simp [isDigitBase10, h])
+  else
+    isFalse (by simp [isDigitBase10, h])
+
+end Char
+
+/-
+TODO: Remove if not needed
+-/
+namespace String
+
+def parseForNatBase10 (str : String) : ParserResult Nat :=
+
+  let rec listToNatBase10Helper : (List Char) → Nat → Nat → ParserResult Nat
+  | [], acc, _ => .success acc
+  | c::cs, acc, pos =>
+    match c.parseForNatBase10 with
+    | .success n => listToNatBase10Helper cs (acc * 10 + n) (pos + 1)
+    | .failure e => .failure {message := e.message, position := e.position}
+
+  match str with
+  | "" =>
+    .failure {
+      message := "input must not be empty"
+      position := 0,
+      input := str
+    }
+  | s  =>
+    match listToNatBase10Helper s.data 0 0 with
+    | .success n => .success n
+    | .failure e => .failure {message := e.message, position := e.position, input := str}
+
+def hasOnlyDigitsBase10 (str : String) : Bool := str.parseForNatBase10.isSuccess
+
+theorem lemma_parse_for_nat_base10 {str : String} :
+  str.hasOnlyDigitsBase10 → str.parseForNatBase10.isSuccess := by
+  intro h
+  unfold hasOnlyDigitsBase10 at h
+  exact h
+
+def parseForNatBase10Guarded (str : String) (g : str.hasOnlyDigitsBase10): Nat :=
+  match h: str.parseForNatBase10 with
+  | .success n => n
+  | .failure _ => by
+      have i : str.parseForNatBase10.isSuccess := by apply lemma_parse_for_nat_base10 g
+      simp [ParserResult.isSuccess] at i
+      grind only
+
+end String
